StandardLibrary/src/MemoryMath.dfy
@@ -8,23 +8,22 @@
 
 
 include "../../libraries/src/BoundedInts.dfy"
+include "UInt.dfy"
 
 module {:options "--function-syntax:4"} MemoryMath {
-  import opened BoundedInts
+  import opened StandardLibrary.UInt
 
   // This is safe because it is being held in memory
   lemma {:axiom} ValueIsSafeBecauseItIsInMemory(value : nat)
-    ensures value < UINT64_MAX as nat
+    ensures HasUint64Size(value)
 
   lemma SequenceIsSafeBecauseItIsInMemory<T>(value : seq<T>)
-    ensures |value| < UINT64_MAX as nat
+    ensures HasUint64Len(value)
   {
     ValueIsSafeBecauseItIsInMemory(|value|);
   }
 
-
   function {:opaque} Add(x : uint64, y : uint64) : (ret : uint64)
-    ensures ret < UINT64_MAX as uint64
     ensures ret as nat == x as nat + y as nat
   {
     ValueIsSafeBecauseItIsInMemory(x as nat + y as nat);
@@ -32,10 +31,52 @@ module {:options "--function-syntax:4"} MemoryMath {
   }
 
   function {:opaque} Add3(x : uint64, y : uint64, z : uint64) : (ret : uint64)
-    ensures ret < UINT64_MAX as uint64
     ensures ret as nat == x as nat + y as nat + z as nat
   {
     ValueIsSafeBecauseItIsInMemory(x as nat + y as nat + z as nat);
     x + y + z
   }
+
+  function {:opaque} Add4(w : uint64, x : uint64, y : uint64, z : uint64) : (ret : uint64)
+    ensures ret as nat == w as nat + x as nat + y as nat + z as nat
+  {
+    ValueIsSafeBecauseItIsInMemory(w as nat + x as nat + y as nat + z as nat);
+    w + x + y + z
+  }
+
+  function {:opaque} Concat<T>(x : seq<T>, y : seq<T>) : (ret : seq64<T>)
+    ensures ret == x + y
+  {
+    SequenceIsSafeBecauseItIsInMemory(x + y);
+    x + y
+  }
+
+  function {:opaque} Concat3<T>(x : seq<T>, y : seq<T>, z : seq<T>) : (ret : seq64<T>)
+    ensures ret == x + y + z
+  {
+    SequenceIsSafeBecauseItIsInMemory(x + y + z);
+    x + y + z
+  }
+
+  function {:opaque} Concat4<T>(w : seq<T>, x : seq<T>, y : seq<T>, z : seq<T>) : (ret : seq64<T>)
+    ensures ret == w + x + y + z
+  {
+    SequenceIsSafeBecauseItIsInMemory(w + x + y + z);
+    w + x + y + z
+  }
+
+  function {:opaque} Concat5<T>(v : seq<T>, w : seq<T>, x : seq<T>, y : seq<T>, z : seq<T>) : (ret : seq64<T>)
+    ensures ret == v + w + x + y + z
+  {
+    SequenceIsSafeBecauseItIsInMemory(v + w + x + y + z);
+    v + w + x + y + z
+  }
+
+  function {:opaque} Concat6<T>(u : seq<T>, v : seq<T>, w : seq<T>, x : seq<T>, y : seq<T>, z : seq<T>) : (ret : seq64<T>)
+    ensures ret == u + v + w + x + y + z
+  {
+    SequenceIsSafeBecauseItIsInMemory(u + v + w + x + y + z);
+    u + v + w + x + y + z
+  }
+
 }
